Christmas commit. :-)
I'm having hard times with these theories. It is
really big and my laptop is really hot and not
going much further in the proofs. I'm getting Exception Size Error
I was suggested by Makarius to use the 2016-1 version with 64bit
enabled. At least I god rid of the exception.

Now he suggested me to rethink about the implementation, because
the translation too direct might be unfeasible. So I'm trying to
make a subset of the entire AST/omega functions trying to identify
how far can we go with the current version of our translation.

I'm posting a brief explanation of our work to the Isabelle mailing
list hoping for some feedback from the experts.

Ho! Ho! Ho!

DefSets.lhs
@@ -1096,3 +1096,8 @@ filter_types_universe ((a,b,c,d):xs) = ((b,b,c,d):(filter_types_universe xs))
 \end{code}
 
 
+\begin{code}
+remdups :: [a] => [a]
+remdups [] = []
+remdups (x:xs) = (if member(x,xs) then remdups xs else x : remdups xs)
+\end{code}
