test_haskabelle/haskabelle/TestingStatelessCircus.thy
@@ -4,7 +4,9 @@ begin
  
 fun omega_CAction :: "((ZName * ZVar) * ZExpr) list \<Rightarrow> CAction \<Rightarrow> CAction"
 where
-  "omega_CAction lst CSPSkip = CSPSkip"
+
+ "omega_CAction lst (CSPRecursion x c) = (CSPRecursion x (omega_CAction lst c))"
+| "omega_CAction lst CSPSkip = CSPSkip"
 | "omega_CAction lst CSPChaos = CSPChaos"
 | "omega_CAction lst CSPStop = CSPStop"
 | "omega_CAction lst (CActionCommand (CAssign va vb)) = (CActionCommand (CAssign va vb))"
@@ -17,6 +19,8 @@ where
 | "omega_CAction lst (CActionCommand (CValDecl va vb)) = (CActionCommand (CValDecl va vb))"
 | "omega_CAction lst (CActionCommand (CVarDecl va vb)) = (CActionCommand (CVarDecl va vb))"
 | "omega_CAction lst (CActionCommand (CVResDecl va vb)) = (CActionCommand (CVResDecl va vb))"
+| "omega_CAction lst (CActionCommand (CommandBrace g)) = undefined"
+| "omega_CAction lst (CActionCommand (CommandBracket g)) = omega_CAction lst (CActionCommand (CPrefix1 g))"
 | "omega_CAction lst (CActionName v) = (CActionName v)"
 | "omega_CAction lst (CActionSchemaExpr v) = (CActionSchemaExpr v)"
 | "omega_CAction lst (CSPCommAction (ChanComm vb (ChanDotExp vc # ve)) va) = (CSPCommAction (ChanComm vb (ChanDotExp vc # ve)) va)"
@@ -39,21 +43,29 @@ where
 | "omega_CAction lst (CSPRepParalNS v va vb vc) = (CSPRepParalNS v va vb vc)"
 | "omega_CAction lst (CSPRepSeq v va) = (CSPRepSeq v va)"
 | "omega_CAction lst (CSPUnParAction v va vb) = (CSPUnParAction v va vb)"
-(*| "omega_CAction lst (CActionCommand (CommandBrace g)) = omega_CAction lst (CActionCommand (CPrefix g (ZTrue Nil)))"
-| "omega_CAction lst (CActionCommand (CommandBracket g)) = omega_CAction lst (CActionCommand (CPrefix1 g))"
 | "omega_CAction lst (CSPCommAction (ChanComm c ((ChanOutExp e) # xs)) a) = omega_CAction lst (CSPCommAction (ChanComm c ((ChanDotExp e) # xs)) a)"
 | "omega_CAction lst (CSPCommAction (ChanComm c Nil) a) = (CSPCommAction (ChanComm c Nil) (omega_CAction lst a))"
 | "omega_CAction lst (CSPHide a cs) = (CSPHide (omega_CAction lst a) cs)"
 | "omega_CAction lst (CSPIntChoice ca cb) = (CSPIntChoice (omega_CAction lst ca) (omega_CAction lst cb))"
 | "omega_CAction lst (CSPSeq ca cb) = (CSPSeq (omega_CAction lst ca) (omega_CAction lst cb))"
-| "omega_CAction lst (CSPRecursion x c) = (CSPRecursion x (omega_CAction lst c))"
+(*
+"(\<lambda>p. size (snd p)) <*mlex*> {}"
 *)
  
 fun \<Omega> :: "CAction \<Rightarrow> CAction"
 where
-  "\<Omega> CSPSkip = CSPSkip"
-| "\<Omega> CSPChaos = CSPChaos"
-| "\<Omega> CSPStop = CSPStop"
+"\<Omega> (CSPRecursion x c) = (CSPRecursion x (\<Omega> c))"
+| "\<Omega> (CSPIntChoice ca cb) = (CSPIntChoice (\<Omega> ca) (\<Omega> cb))"
+| "\<Omega> (CSPSeq ca cb) = (CSPSeq (\<Omega> ca) (\<Omega> cb))"
+| "\<Omega> (CSPHide a cs) = (CSPHide (\<Omega> a) cs)"
+| "\<Omega> (CActionName v) = (CActionName v)"
+| "\<Omega> (CActionSchemaExpr v) = (CActionSchemaExpr v)"
+| "\<Omega> (CSPCommAction (ChanComm c ((ChanOutExp e) # xs)) a) = \<Omega> (CSPCommAction (ChanComm c ((ChanDotExp e) # xs)) a)"
+| "\<Omega> (CSPCommAction (ChanComm c Nil) a) = (CSPCommAction (ChanComm c Nil) (\<Omega> a))"
+| "\<Omega> (CSPCommAction (ChanComm vb (ChanDotExp vc # ve)) va) = (CSPCommAction (ChanComm vb (ChanDotExp vc # ve)) va)"
+| "\<Omega> (CSPCommAction (ChanComm vb (ChanInp vc # ve)) va) = (CSPCommAction (ChanComm vb (ChanInp vc # ve)) va)"
+| "\<Omega> (CSPCommAction (ChanComm vb (ChanInpPred v vc # ve)) va) = (CSPCommAction (ChanComm vb (ChanInpPred v vc # ve)) va)"
+| "\<Omega> (CSPCommAction (ChanGenComm vb vc vd) va) = (CSPCommAction (ChanGenComm vb vc vd) va)"
 | "\<Omega> (CActionCommand (CAssign va vb)) = (CActionCommand (CAssign va vb))"
 | "\<Omega> (CActionCommand (CAssumpt va vb vc)) = (CActionCommand (CAssumpt va vb vc))"
 | "\<Omega> (CActionCommand (CAssumpt1 va vb)) = (CActionCommand (CAssumpt1 va vb))"
@@ -64,15 +76,8 @@ where
 | "\<Omega> (CActionCommand (CValDecl va vb)) = (CActionCommand (CValDecl va vb))"
 | "\<Omega> (CActionCommand (CVarDecl va vb)) = (CActionCommand (CVarDecl va vb))"
 | "\<Omega> (CActionCommand (CVResDecl va vb)) = (CActionCommand (CVResDecl va vb))"
-| "\<Omega> (CActionName v) = (CActionName v)"
-| "\<Omega> (CActionSchemaExpr v) = (CActionSchemaExpr v)"
-| "\<Omega> (CSPCommAction (ChanComm vb (ChanDotExp vc # ve)) va) = (CSPCommAction (ChanComm vb (ChanDotExp vc # ve)) va)"
-| "\<Omega> (CSPCommAction (ChanComm vb (ChanInp vc # ve)) va) = (CSPCommAction (ChanComm vb (ChanInp vc # ve)) va)"
-| "\<Omega> (CSPCommAction (ChanComm vb (ChanInpPred v vc # ve)) va) = (CSPCommAction (ChanComm vb (ChanInpPred v vc # ve)) va)"
-| "\<Omega> (CSPCommAction (ChanGenComm vb vc vd) va) = (CSPCommAction (ChanGenComm vb vc vd) va)"
-| "\<Omega> (CSPExtChoice v va) = (CSPExtChoice v va)"
-| "\<Omega> (CSPGuard v va) = (CSPGuard v va)"
-| "\<Omega> (CSPInterleave v va) = (CSPInterleave v va)"
+| "\<Omega> (CActionCommand (CommandBrace g)) = \<Omega> (CActionCommand (CPrefix g (ZTrue Nil)))"
+| "\<Omega> (CActionCommand (CommandBracket g)) = \<Omega> (CActionCommand (CPrefix1 g))"
 | "\<Omega> (CSPNSInter v va vb vc) = (CSPNSInter v va vb vc)"
 | "\<Omega> (CSPNSParal v va vb vc vd) = (CSPNSParal v va vb vc vd)"
 | "\<Omega> (CSPParAction v va) = (CSPParAction v va)"
@@ -86,162 +91,49 @@ where
 | "\<Omega> (CSPRepParalNS v va vb vc) = (CSPRepParalNS v va vb vc)"
 | "\<Omega> (CSPRepSeq v va) = (CSPRepSeq v va)"
 | "\<Omega> (CSPUnParAction v va vb) = (CSPUnParAction v va vb)"
-(*
-| "\<Omega> (CActionCommand (CommandBrace g)) = \<Omega> (CActionCommand (CPrefix g (ZTrue Nil)))"
-| "\<Omega> (CActionCommand (CommandBracket g)) = \<Omega> (CActionCommand (CPrefix1 g))"
-| "\<Omega> (CSPCommAction (ChanComm c ((ChanOutExp e) # xs)) a) = \<Omega> (CSPCommAction (ChanComm c ((ChanDotExp e) # xs)) a)"
-| "\<Omega> (CSPCommAction (ChanComm c Nil) a) = (CSPCommAction (ChanComm c Nil) (\<Omega> a))"
-| "\<Omega> (CSPHide a cs) = (CSPHide (\<Omega> a) cs)"
-| "\<Omega> (CSPIntChoice ca cb) = (CSPIntChoice (\<Omega> ca) (\<Omega> cb))"
-| "\<Omega> (CSPSeq ca cb) = (CSPSeq (\<Omega> ca) (\<Omega> cb))"
-| "\<Omega> (CSPRecursion x c) = (CSPRecursion x (\<Omega> c))"
-*)
- 
-lemma omega_CSPSkip: "omega_CAction lst CSPSkip = (\<Omega> CSPSkip)"
-  by simp
-lemma omega_CSPChaos:"omega_CAction lst CSPChaos = (\<Omega> CSPChaos)"
-  by simp
+| "\<Omega> (CSPExtChoice v va) = (CSPExtChoice v va)"
+| "\<Omega> (CSPGuard v va) = (CSPGuard v va)"
+| "\<Omega> (CSPInterleave v va) = (CSPInterleave v va)"
+| "\<Omega> CSPSkip = CSPSkip"
+| "\<Omega> CSPChaos = CSPChaos"
+| "\<Omega> CSPStop = CSPStop"
 
-lemma omega_CSPStop: "omega_CAction lst CSPStop = (\<Omega> CSPStop)"
-  by simp
+lemma "omega_CAction lst (\<Omega> (CActionSchemaExpr x)) = \<Omega> (omega_CAction lst (CActionSchemaExpr x))"
+oops
 
-lemma omega_CAssign:"omega_CAction lst (CActionCommand (CAssign va vb)) = (\<Omega> (CActionCommand (CAssign va vb)))"
-  by simp
-
-
-lemma omega_CAssumpt:"omega_CAction lst (CActionCommand (CAssumpt va vb vc)) = (\<Omega> (CActionCommand (CAssumpt va vb vc)))"
-  by simp
-
-
-lemma omega_CAssumpt1:"omega_CAction lst (CActionCommand (CAssumpt1 va vb)) = (\<Omega> (CActionCommand (CAssumpt1 va vb)))"
-  by simp
-
-
-lemma omega_CIf:"omega_CAction lst (CActionCommand (CIf a)) = (\<Omega> (CActionCommand (CIf a)))"
-  by simp
-
-
-lemma omega_CPrefix:"omega_CAction lst (CActionCommand (CPrefix va vb)) = (\<Omega> (CActionCommand (CPrefix va vb)))"
-  by simp
+lemma "\<And>x. omega_CAction lst (\<Omega> (CActionCommand x)) = \<Omega> (omega_CAction lst (CActionCommand x))"
+oops
+lemma "\<And>x. omega_CAction lst (\<Omega> (CActionName x)) = \<Omega> (omega_CAction lst (CActionName x))"
+oops
+lemma "omega_CAction lst (\<Omega> CSPSkip) = \<Omega> (omega_CAction lst CSPSkip)"
+oops
+lemma "omega_CAction lst (\<Omega> CSPStop) = \<Omega> (omega_CAction lst CSPStop)"
+oops
+lemma "omega_CAction lst (\<Omega> CSPChaos) = \<Omega> (omega_CAction lst CSPChaos)"
+oops
+lemma "\<And>x1 a. omega_CAction lst (\<Omega> a) = \<Omega> (omega_CAction lst a) \<Longrightarrow>
+            omega_CAction lst (\<Omega> (CSPCommAction x1 a)) = \<Omega> (omega_CAction lst (CSPCommAction x1 a))"
+oops
+lemma "\<And>x1 a. omega_CAction lst (\<Omega> a) = \<Omega> (omega_CAction lst a) \<Longrightarrow>
+            omega_CAction lst (\<Omega> (CSPGuard x1 a)) = \<Omega> (omega_CAction lst (CSPGuard x1 a))"
+oops
+lemma "\<And>a1 a2. omega_CAction lst (\<Omega> a1) = \<Omega> (omega_CAction lst a1) \<Longrightarrow>
+             omega_CAction lst (\<Omega> a2) = \<Omega> (omega_CAction lst a2) \<Longrightarrow>
+             omega_CAction lst (\<Omega> (CSPSeq a1 a2)) = \<Omega> (omega_CAction lst (CSPSeq a1 a2))"
+oops
+lemma "\<And>a1 a2. omega_CAction lst (\<Omega> a1) = \<Omega> (omega_CAction lst a1) \<Longrightarrow>
+              omega_CAction lst (\<Omega> a2) = \<Omega> (omega_CAction lst a2) \<Longrightarrow>
+              omega_CAction lst (\<Omega> (CSPExtChoice a1 a2)) = \<Omega> (omega_CAction lst (CSPExtChoice a1 a2))"
+oops
 
 
-lemma omega_CPrefix1: "omega_CAction lst (CActionCommand (CPrefix1 va)) = (\<Omega> (CActionCommand (CPrefix1 va)))"
-  by simp
-
-
-lemma omega_CResDecl: "omega_CAction lst (CActionCommand (CResDecl va vb)) = (\<Omega> (CActionCommand (CResDecl va vb)))"
-  by simp
-
-
-lemma omega_CValDecl: "omega_CAction lst (CActionCommand (CValDecl va vb)) = (\<Omega> (CActionCommand (CValDecl va vb)))"
-  by simp
-
-
-lemma omega_CVarDecl: "omega_CAction lst (CActionCommand (CVarDecl va vb)) = (\<Omega> (CActionCommand (CVarDecl va vb)))"
-  by simp
-
-
-lemma omega_CVResDecl: "omega_CAction lst (CActionCommand (CVResDecl va vb)) = (\<Omega> (CActionCommand (CVResDecl va vb)))"
-  by simp
-
-
-lemma omega_CActionName: "omega_CAction lst (CActionName v) = (\<Omega> (CActionName v))"
-  by simp
-
-
-lemma omega_CActionSchemaExpr: "omega_CAction lst (CActionSchemaExpr v) = (\<Omega> (CActionSchemaExpr v))"
-  by simp
-
-
-lemma omega_CSPCommActionChanDotExp: "omega_CAction lst (CSPCommAction (ChanComm vb (ChanDotExp vc # ve)) va) = (\<Omega> (CSPCommAction (ChanComm vb (ChanDotExp vc # ve)) va))"
-  by simp
-
-lemma omega_CSPCommActionChanInp: "omega_CAction lst (CSPCommAction (ChanComm vb (ChanInp vc # ve)) va) = (\<Omega> (CSPCommAction (ChanComm vb (ChanInp vc # ve)) va))"
-  by simp
-
-lemma omega_CSPCommActionChanInpPred: "omega_CAction lst (CSPCommAction (ChanComm vb (ChanInpPred v vc # ve)) va) = (\<Omega> (CSPCommAction (ChanComm vb (ChanInpPred v vc # ve)) va))"
-  by simp
-
-lemma omega_CSPCommActionChanGenComm: "omega_CAction lst (CSPCommAction (ChanGenComm vb vc vd) va) = (\<Omega> (CSPCommAction (ChanGenComm vb vc vd) va))"
-  by simp
-
-
-lemma omega_CSPExtChoice: "omega_CAction lst (CSPExtChoice v va) = (\<Omega> (CSPExtChoice v va))"
-  by simp
-
-
-lemma omega_CSPGuard: "omega_CAction lst (CSPGuard v va) = (\<Omega> (CSPGuard v va))"
-  by simp
-
-
-lemma omega_CSPInterleave: "omega_CAction lst (CSPInterleave v va) = (\<Omega> (CSPInterleave v va))"
-  by simp
-
-
-lemma omega_CSPNSInter: "omega_CAction lst (CSPNSInter v va vb vc) = (\<Omega> (CSPNSInter v va vb vc))"
-  by simp
-
-
-lemma omega_CSPNSParal: "omega_CAction lst (CSPNSParal v va vb vc vd) = (\<Omega> (CSPNSParal v va vb vc vd))"
-  by simp
-
-
-lemma omega_CSPParAction: "omega_CAction lst (CSPParAction v va) = (\<Omega> (CSPParAction v va))"
-  by simp
-
-
-lemma omega_CSPParal: "omega_CAction lst (CSPParal v va vb) = (\<Omega> (CSPParal v va vb))"
-  by simp
-
-
-lemma omega_CSPRenAction: "omega_CAction lst (CSPRenAction v va) = (\<Omega> (CSPRenAction v va))"
-  by simp
-
-
-lemma omega_CSPRepExtChoice: "omega_CAction lst (CSPRepExtChoice v va) = (\<Omega> (CSPRepExtChoice v va))"
-  by simp
-
-
-lemma omega_CSPRepIntChoice: "omega_CAction lst (CSPRepIntChoice v va) = (\<Omega> (CSPRepIntChoice v va))"
-  by simp
-
-
-lemma omega_CSPRepInterl: "omega_CAction lst (CSPRepInterl v va) = (\<Omega> (CSPRepInterl v va))"
-  by simp
-
-
-lemma omega_CSPRepParal: "omega_CAction lst (CSPRepInterlNS v va vb) = (\<Omega> (CSPRepInterlNS v va vb))"
-  by simp
-
-
-lemma "omega_CAction lst (CSPRepParal v va vb) = (\<Omega> (CSPRepParal v va vb))"
-  by simp
-
-
-lemma omega_CSPRepParalNS: "omega_CAction lst (CSPRepParalNS v va vb vc) = (\<Omega> (CSPRepParalNS v va vb vc))"
-  by simp
-
-
-lemma omega_CSPRepSeq: "omega_CAction lst (CSPRepSeq v va) = (\<Omega> (CSPRepSeq v va))"
-  by simp
-
-
-lemma omega_CSPUnParAction: "omega_CAction lst (CSPUnParAction v va vb) = (\<Omega> (CSPUnParAction v va vb))"
-  by simp
-
-lemma "length(tl xs) = length xs - 1" 
-  proof (cases xs)
-    assume "xs = []"
-    thus ?thesis by simp 
-  next
-    fix y ys assume "xs = y#ys"
-    thus ?thesis by simp 
-qed
+lemma "omega_CAction lst (\<Omega> a) = (\<Omega> (omega_CAction lst a))"
+    apply (induction a)
+    apply auto
+    apply sledgehammer
 
 lemma "omega_CAction lst a = (\<Omega> a)"
-    proof (cases a)
-      assume "\<And>x1. a = CActionSchemaExpr x1"
-      
-       
-  
+    apply (induction a rule: \<Omega>.induct)
+    apply auto
+sorry
 end
