test_haskabelle/haskabelle/AST.thy
@@ -14,70 +14,6 @@ type_synonym GivenSet = ZVar
  
 type_synonym ZName = string
  
-fun make_zvar :: "string \<Rightarrow> ZDecor list \<Rightarrow> ZVar"
-where
-  "make_zvar s dl = (s, dl)"
-
- 
-fun decorate_zvar :: "ZVar \<Rightarrow> ZDecor list \<Rightarrow> ZVar"
-where
-  "decorate_zvar (s, dl) d = (s, (dl @ d))"
-
- 
-fun prime_zvar :: "ZVar \<Rightarrow> ZVar"
-where
-  "prime_zvar v = decorate_zvar v [''''']"
-
- 
-fun unprime_zvar :: "ZVar \<Rightarrow> ZVar"
-where
-  "unprime_zvar (n, [''''']) = (n, Nil)"
-
- 
-fun string_to_zvar :: "string \<Rightarrow> ZVar"
-where
-  "string_to_zvar s = make_zvar s Nil"
-
- 
-definition get_zvar_name :: "ZVar \<Rightarrow> string"
-where
-  "get_zvar_name = fst"
-
- 
-definition get_zvar_decor :: "ZVar \<Rightarrow> ZDecor list"
-where
-  "get_zvar_decor = snd"
-
- 
-fun is_unprimed_zvar :: "ZVar \<Rightarrow> bool"
-where
-  "is_unprimed_zvar (_, Nil) = True"
-| "is_unprimed_zvar _ = False"
-
- 
-fun is_primed_zvar :: "ZVar \<Rightarrow> bool"
-where
-  "is_primed_zvar (_, [''''']) = True"
-| "is_primed_zvar _ = False"
-
- 
-fun is_input_zvar :: "ZVar \<Rightarrow> bool"
-where
-  "is_input_zvar (_, [''?'']) = True"
-| "is_input_zvar _ = False"
-
- 
-fun is_output_zvar :: "ZVar \<Rightarrow> bool"
-where
-  "is_output_zvar (_, [''!'']) = True"
-| "is_output_zvar _ = False"
-
- 
-fun show_zvar :: "ZVar \<Rightarrow> string"
-where
-  "show_zvar (s, dl) = (s @ concat dl)"
-
- 
 datatype ZReln = ZLessThan
                | ZLessThanEq
                | ZGreaterThan
@@ -217,199 +153,10 @@ and      ZReplace = ZRename ZVar ZVar
 and      ZBranch = ZBranch0 ZVar
                  | ZBranch1 ZVar ZExpr
  
-primrec baseset :: "ZExpr \<Rightarrow> ZExpr"
-where
-  "baseset (ZPowerSet x _ _) = x"
-
- 
-primrec is_non_empty :: "ZExpr \<Rightarrow> bool"
-where
-  "is_non_empty (ZFuncSet _ _ _ _ _ _ _ x _) = x"
-| "is_non_empty (ZPowerSet _ x _) = x"
-
- 
-primrec is_finite :: "ZExpr \<Rightarrow> bool"
-where
-  "is_finite (ZFuncSet _ _ _ _ _ _ _ _ x) = x"
-| "is_finite (ZPowerSet _ _ x) = x"
-
- 
-primrec domset :: "ZExpr \<Rightarrow> ZExpr"
-where
-  "domset (ZFuncSet x _ _ _ _ _ _ _ _) = x"
-
- 
-primrec ranset :: "ZExpr \<Rightarrow> ZExpr"
-where
-  "ranset (ZFuncSet _ x _ _ _ _ _ _ _) = x"
-
- 
-primrec is_function :: "ZExpr \<Rightarrow> bool"
-where
-  "is_function (ZFuncSet _ _ x _ _ _ _ _ _) = x"
-
- 
-primrec is_total :: "ZExpr \<Rightarrow> bool"
-where
-  "is_total (ZFuncSet _ _ _ x _ _ _ _ _) = x"
-
- 
-primrec is_onto :: "ZExpr \<Rightarrow> bool"
-where
-  "is_onto (ZFuncSet _ _ _ _ x _ _ _ _) = x"
-
- 
-primrec is_one2one :: "ZExpr \<Rightarrow> bool"
-where
-  "is_one2one (ZFuncSet _ _ _ _ _ x _ _ _) = x"
-
- 
-primrec is_sequence :: "ZExpr \<Rightarrow> bool"
-where
-  "is_sequence (ZFuncSet _ _ _ _ _ _ x _ _) = x"
-
- 
-primrec update_baseset :: "ZExpr \<Rightarrow> ZExpr \<Rightarrow> ZExpr"
-where
-  "update_baseset x (ZPowerSet _ f2 f3) = (ZPowerSet x f2 f3)"
-
- 
-primrec update_is_non_empty :: "bool \<Rightarrow> ZExpr \<Rightarrow> ZExpr"
-where
-  "update_is_non_empty x (ZFuncSet f1 f2 f3 f4 f5 f6 f7 _ f9) = (ZFuncSet f1 f2 f3 f4 f5 f6 f7 x f9)"
-| "update_is_non_empty x (ZPowerSet f1 _ f3) = (ZPowerSet f1 x f3)"
-
- 
-primrec update_is_finite :: "bool \<Rightarrow> ZExpr \<Rightarrow> ZExpr"
-where
-  "update_is_finite x (ZFuncSet f1 f2 f3 f4 f5 f6 f7 f8 _) = (ZFuncSet f1 f2 f3 f4 f5 f6 f7 f8 x)"
-| "update_is_finite x (ZPowerSet f1 f2 _) = (ZPowerSet f1 f2 x)"
-
- 
-primrec update_domset :: "ZExpr \<Rightarrow> ZExpr \<Rightarrow> ZExpr"
-where
-  "update_domset x (ZFuncSet _ f2 f3 f4 f5 f6 f7 f8 f9) = (ZFuncSet x f2 f3 f4 f5 f6 f7 f8 f9)"
-
- 
-primrec update_ranset :: "ZExpr \<Rightarrow> ZExpr \<Rightarrow> ZExpr"
-where
-  "update_ranset x (ZFuncSet f1 _ f3 f4 f5 f6 f7 f8 f9) = (ZFuncSet f1 x f3 f4 f5 f6 f7 f8 f9)"
-
- 
-primrec update_is_function :: "bool \<Rightarrow> ZExpr \<Rightarrow> ZExpr"
-where
-  "update_is_function x (ZFuncSet f1 f2 _ f4 f5 f6 f7 f8 f9) = (ZFuncSet f1 f2 x f4 f5 f6 f7 f8 f9)"
-
- 
-primrec update_is_total :: "bool \<Rightarrow> ZExpr \<Rightarrow> ZExpr"
-where
-  "update_is_total x (ZFuncSet f1 f2 f3 _ f5 f6 f7 f8 f9) = (ZFuncSet f1 f2 f3 x f5 f6 f7 f8 f9)"
-
- 
-primrec update_is_onto :: "bool \<Rightarrow> ZExpr \<Rightarrow> ZExpr"
-where
-  "update_is_onto x (ZFuncSet f1 f2 f3 f4 _ f6 f7 f8 f9) = (ZFuncSet f1 f2 f3 f4 x f6 f7 f8 f9)"
-
- 
-primrec update_is_one2one :: "bool \<Rightarrow> ZExpr \<Rightarrow> ZExpr"
-where
-  "update_is_one2one x (ZFuncSet f1 f2 f3 f4 f5 _ f7 f8 f9) = (ZFuncSet f1 f2 f3 f4 f5 x f7 f8 f9)"
-
- 
-primrec update_is_sequence :: "bool \<Rightarrow> ZExpr \<Rightarrow> ZExpr"
-where
-  "update_is_sequence x (ZFuncSet f1 f2 f3 f4 f5 f6 _ f8 f9) = (ZFuncSet f1 f2 f3 f4 f5 f6 x f8 f9)"
-
- 
-primrec reason :: "ZPred \<Rightarrow> ZPred list"
-where
-  "reason (ZTrue x) = x"
-| "reason (ZFalse x) = x"
-
- 
-primrec update_reason :: "ZPred list \<Rightarrow> ZPred \<Rightarrow> ZPred"
-where
-  "update_reason x (ZTrue _) = (ZTrue x)"
-| "update_reason x (ZFalse _) = (ZFalse x)"
-
- 
-fun genfilt_names :: "ZGenFilt list \<Rightarrow> ZVar list"
-where
-  "genfilt_names Nil = Nil"
-| "genfilt_names (Choose v _ # gfs) = (v # genfilt_names gfs)"
-| "genfilt_names (Check _ # gfs) = genfilt_names gfs"
-| "genfilt_names (Evaluate v _ _ # gfs) = (v # genfilt_names gfs)"
-| "genfilt_names (Include s # gfs) = error (''genfilt_names called before '' @ (print s @ '' expanded.''))"
-
  
 type_synonym ZValue = ZExpr
  
-fun is_pair :: "ZValue \<Rightarrow> bool"
-where
-  "is_pair (ZTuple [_, _]) = True"
-| "is_pair _ = False"
-
- 
-fun pair_fst :: "ZValue \<Rightarrow> ZValue"
-where
-  "pair_fst (ZTuple [x, _]) = x"
-| "pair_fst _ = error ''pair_fst applied to non-pair value''"
-
- 
-fun pair_snd :: "ZValue \<Rightarrow> ZValue"
-where
-  "pair_snd (ZTuple [_, y]) = y"
-| "pair_snd _ = error ''pair_snd applied to non-pair value''"
-
- 
-definition zrelations :: "ZExpr"
-where
-  "zrelations = ZFuncSet ZUniverse ZUniverse False False False False False False False"
-
- 
-definition ztrue
-where
-  "ztrue = ZTrue Nil"
-
- 
-definition zfalse
-where
-  "zfalse = ZFalse Nil"
-
- 
-fun isBranch0 :: "ZBranch \<Rightarrow> bool"
-where
-  "isBranch0 (ZBranch0 _) = True"
-| "isBranch0 _ = False"
-
- 
-fun isCanonical :: "ZExpr \<Rightarrow> bool"
-where
-  "isCanonical (ZInt _) = True"
-| "isCanonical (ZTuple v) = list_all isCanonical v"
-| "isCanonical (ZGiven _) = True"
-| "isCanonical (ZFree0 _) = True"
-| "isCanonical (ZFree1 _ v) = isCanonical v"
-| "isCanonical (ZBinding bs) = list_all (isCanonical o snd) bs"
-| "isCanonical _ = False"
-
- 
-fun isDefined :: "ZExpr \<Rightarrow> bool"
-where
-  "isDefined (ZInt _) = True"
-| "isDefined (ZIntSet _ _) = True"
-| "isDefined (ZTuple v) = list_all isDefined v"
-| "isDefined (ZReln _) = True"
-| "isDefined (ZGiven _) = True"
-| "isDefined (ZGivenSet _) = True"
-| "isDefined (ZSetDisplay vs) = list_all isDefined vs"
-| "isDefined (ZSeqDisplay vs) = list_all isDefined vs"
-| "isDefined (ZFree0 _) = True"
-| "isDefined (ZFree1 _ _) = True"
-| "isDefined (ZBinding bs) = list_all (isDefined o snd) bs"
-| "isDefined v = False"
-
- 
+(* 
 datatype CDecl = CChan ZName
                | CChanDecl ZName ZExpr
                | CGenChanDecl ZName ZName ZExpr
@@ -428,7 +175,7 @@ datatype NSExp = NSExpEmpty
                | NSUnion NSExp NSExp
                | NSIntersect NSExp NSExp
                | NSHide NSExp NSExp
-               | NSBigUnion ZExpr
+               | NSBigUnion ZExpr*)
  
 datatype CParameter = ChanInp ZName
                     | ChanInpPred ZName ZPred
@@ -442,16 +189,16 @@ datatype CReplace = CRename "ZVar list" "ZVar list"
                   | CRenameAssign "ZVar list" "ZVar list"
  
 datatype ParAction = CircusAction CAction
-                   | ParamActionDecl "ZGenFilt list" ParAction
-and      CAction = CActionSchemaExpr ZSExpr
+                  (* | ParamActionDecl "ZGenFilt list" ParAction*)
+and      CAction = (*CActionSchemaExpr ZSExpr
                  | CActionCommand CCommand
-                 | CActionName ZName
-                 | CSPSkip
+                 | CActionName ZName*)
+                  CSPSkip
                  | CSPStop
                  | CSPChaos
                  | CSPCommAction Comm CAction
-                 | CSPGuard ZPred CAction
                  | CSPSeq CAction CAction
+                (* | CSPGuard ZPred CAction
                  | CSPExtChoice CAction CAction
                  | CSPIntChoice CAction CAction
                  | CSPNSParal NSExp CSExp NSExp CAction CAction
@@ -459,18 +206,18 @@ and      CAction = CActionSchemaExpr ZSExpr
                  | CSPNSInter NSExp NSExp CAction CAction
                  | CSPInterleave CAction CAction
                  | CSPHide CAction CSExp
-                 | CSPParAction ZName "ZExpr list"
-                 | CSPRenAction ZName CReplace
+                 *)| CSPParAction ZName "ZExpr list"
+                 (*| CSPRenAction ZName CReplace
                  | CSPRecursion ZName CAction
-                 | CSPUnParAction "ZGenFilt list" CAction ZName
+                 | CSPUnParAction "ZGenFilt list" CAction ZName*)
                  | CSPRepSeq "ZGenFilt list" CAction
-                 | CSPRepExtChoice "ZGenFilt list" CAction
+                (* | CSPRepExtChoice "ZGenFilt list" CAction
                  | CSPRepIntChoice "ZGenFilt list" CAction
                  | CSPRepParalNS CSExp "ZGenFilt list" NSExp CAction
                  | CSPRepParal CSExp "ZGenFilt list" CAction
                  | CSPRepInterlNS "ZGenFilt list" NSExp CAction
-                 | CSPRepInterl "ZGenFilt list" CAction
-and      CCommand = CAssign "ZVar list" "ZExpr list"
+                 | CSPRepInterl "ZGenFilt list" CAction*)
+(*and      CCommand = CAssign "ZVar list" "ZExpr list"
                   | CIf CGActions
                   | CVarDecl "ZGenFilt list" CAction
                   | CAssumpt "ZName list" ZPred ZPred
@@ -484,8 +231,8 @@ and      CCommand = CAssign "ZVar list" "ZExpr list"
                   | CVResDecl "ZGenFilt list" CAction
 and      CGActions = CircGAction ZPred CAction
                    | CircThenElse CGActions CGActions
-                   | CircElse ParAction
- 
+                   | CircElse ParAction*)
+ (*
 datatype ZPara = ZGivenSetDecl GivenSet
                | ZSchemaDef ZSName ZSExpr
                | ZAbbreviation ZVar ZExpr
@@ -524,157 +271,7 @@ and      CProc = CRepSeqProc "ZGenFilt list" CProc
 and      PPar = ProcZPara ZPara
               | CParAction ZName ParAction
               | CNameSet ZName NSExp
- 
-primrec machName :: "ZPara \<Rightarrow> string"
-where
-  "machName (ZMachineDef x _ _ _) = x"
-
- 
-primrec machState :: "ZPara \<Rightarrow> string"
-where
-  "machState (ZMachineDef _ x _ _) = x"
-
- 
-primrec machInit :: "ZPara \<Rightarrow> string"
-where
-  "machInit (ZMachineDef _ _ x _) = x"
-
- 
-primrec machOps :: "ZPara \<Rightarrow> string list"
-where
-  "machOps (ZMachineDef _ _ _ x) = x"
-
- 
-primrec update_machName :: "string \<Rightarrow> ZPara \<Rightarrow> ZPara"
-where
-  "update_machName x (ZMachineDef _ f2 f3 f4) = (ZMachineDef x f2 f3 f4)"
-
- 
-primrec update_machState :: "string \<Rightarrow> ZPara \<Rightarrow> ZPara"
-where
-  "update_machState x (ZMachineDef f1 _ f3 f4) = (ZMachineDef f1 x f3 f4)"
-
- 
-primrec update_machInit :: "string \<Rightarrow> ZPara \<Rightarrow> ZPara"
-where
-  "update_machInit x (ZMachineDef f1 f2 _ f4) = (ZMachineDef f1 f2 x f4)"
-
- 
-primrec update_machOps :: "string list \<Rightarrow> ZPara \<Rightarrow> ZPara"
-where
-  "update_machOps x (ZMachineDef f1 f2 f3 _) = (ZMachineDef f1 f2 f3 x)"
-
- 
-type_synonym ZSpec = "ZPara list"
- 
-type_synonym CProgram = "ZPara list"
- 
-type_synonym SearchSpace = "(ZVar * int) list"
- 
-type_synonym GlobalDefs = "(ZVar * ZExpr) list"
- 
-datatype Env = Env int SearchSpace int int GlobalDefs "(ZVar * ZExpr) list"
- 
-primrec search_space :: "Env \<Rightarrow> int"
-where
-  "search_space (Env x _ _ _ _ _) = x"
-
- 
-primrec search_vars :: "Env \<Rightarrow> SearchSpace"
-where
-  "search_vars (Env _ x _ _ _ _) = x"
-
- 
-primrec max_search_space :: "Env \<Rightarrow> int"
-where
-  "max_search_space (Env _ _ x _ _ _) = x"
-
- 
-primrec max_set_size :: "Env \<Rightarrow> int"
-where
-  "max_set_size (Env _ _ _ x _ _) = x"
-
- 
-primrec global_values :: "Env \<Rightarrow> GlobalDefs"
-where
-  "global_values (Env _ _ _ _ x _) = x"
-
- 
-primrec local_values :: "Env \<Rightarrow> (ZVar * ZExpr) list"
-where
-  "local_values (Env _ _ _ _ _ x) = x"
-
- 
-primrec update_search_space :: "int \<Rightarrow> Env \<Rightarrow> Env"
-where
-  "update_search_space x (Env _ f2 f3 f4 f5 f6) = (Env x f2 f3 f4 f5 f6)"
-
- 
-primrec update_search_vars :: "SearchSpace \<Rightarrow> Env \<Rightarrow> Env"
-where
-  "update_search_vars x (Env f1 _ f3 f4 f5 f6) = (Env f1 x f3 f4 f5 f6)"
-
- 
-primrec update_max_search_space :: "int \<Rightarrow> Env \<Rightarrow> Env"
-where
-  "update_max_search_space x (Env f1 f2 _ f4 f5 f6) = (Env f1 f2 x f4 f5 f6)"
-
- 
-primrec update_max_set_size :: "int \<Rightarrow> Env \<Rightarrow> Env"
-where
-  "update_max_set_size x (Env f1 f2 f3 _ f5 f6) = (Env f1 f2 f3 x f5 f6)"
-
- 
-primrec update_global_values :: "GlobalDefs \<Rightarrow> Env \<Rightarrow> Env"
-where
-  "update_global_values x (Env f1 f2 f3 f4 _ f6) = (Env f1 f2 f3 f4 x f6)"
-
- 
-primrec update_local_values :: "(ZVar * ZExpr) list \<Rightarrow> Env \<Rightarrow> Env"
-where
-  "update_local_values x (Env f1 f2 f3 f4 f5 _) = (Env f1 f2 f3 f4 f5 x)"
-
- 
-fun empty_env :: "GlobalDefs \<Rightarrow> Env"
-where
-  "empty_env gdefs = Env 1 Nil 100000 1000 gdefs Nil"
-
- 
-definition dummy_eval_env
-where
-  "dummy_eval_env = (update_max_search_space 10000) (empty_env Nil)"
-
- 
-fun set_max_search_space :: "int \<Rightarrow> Env \<Rightarrow> Env"
-where
-  "set_max_search_space i env = (update_max_search_space i) env"
-
- 
-fun set_max_set_size :: "int \<Rightarrow> Env \<Rightarrow> Env"
-where
-  "set_max_set_size i env = (update_max_set_size i) env"
-
- 
-fun envPushLocal :: "ZVar \<Rightarrow> ZExpr \<Rightarrow> Env \<Rightarrow> Env"
-where
-  "envPushLocal v val env = (update_local_values ((v, val) # local_values env)) env"
-
- 
-fun envPushLocals :: "(ZVar * ZExpr) list \<Rightarrow> Env \<Rightarrow> Env"
-where
-  "envPushLocals vs env = (update_local_values (vs @ local_values env)) env"
-
- 
-fun envIsLocal :: "Env \<Rightarrow> ZVar \<Rightarrow> bool"
-where
-  "envIsLocal env v = member v (map fst (local_values env))"
-
- 
-fun envIsSchema :: "Env \<Rightarrow> string \<Rightarrow> bool"
-where
-  "envIsSchema env v = Not (null ([0 . (n, (ZESchema _)) <- global_values env,
-                                       eq n (string_to_zvar v)]))"
-
+ *)
  
 datatype ZTerm = ZExpr ZExpr
                | ZPred ZPred
